ulib/LowStar.RST.Pointer.fst
@@ -24,7 +24,9 @@ module Seq = FStar.Seq
 open LowStar.RST
 open LowStar.BufferOps
 
+abstract
 let ptr_view (#a:Type) (ptr:B.pointer a) : view a = 
+  reveal_view ();
   let fp = Ghost.hide (B.loc_buffer ptr) in 
   let inv h = B.live h ptr in
   let sel h = Seq.index (B.as_seq h ptr) 0 in
@@ -44,7 +46,7 @@ let reveal_ptr ()
              inv (ptr_resource ptr) h <==> B.live h ptr) /\
            (forall a (ptr:B.pointer a) h .{:pattern sel (ptr_view ptr) h} 
              sel (ptr_view ptr) h == Seq.index (B.as_seq h ptr) 0)) = 
-  reveal ()
+  ()
 
 let ptr_read (#a:Type)
              (ptr:B.pointer a)
@@ -54,7 +56,6 @@ let ptr_read (#a:Type)
                    (fun h0 x h1 -> 
                       sel (ptr_view ptr) h0 == x /\ 
                       x == sel (ptr_view ptr) h1) =
-  reveal ();
   !* ptr
 
 let ptr_write (#a:Type)
@@ -65,5 +66,5 @@ let ptr_write (#a:Type)
                        (fun _ -> True)
                        (fun _ _ h1 -> 
                           sel (ptr_view ptr) h1 == x) =
-  reveal ();
+  reveal_modifies ();
   ptr *= x
